Proved act_sample.

examples/sampler/verif_sampler.v
@@ -5,6 +5,8 @@ Require Import Poulet4.P4light.Architecture.Tofino.
 Require Import ProD3.core.Tofino.
 Require Import ProD3.examples.sampler.common.
 Require Import ProD3.examples.sampler.ModelRepr.
+Require Import ProD3.core.ProgNotations.
+Require Import Poulet4.P4light.Syntax.P4Notations.
 Require Import Hammer.Plugin.Hammer.
 Require Export Coq.Program.Program.
 Import ListNotations.
@@ -60,23 +62,96 @@ Qed.
 Definition act_sample_fundef :=
   ltac:(get_fd ["SwitchIngress"; "act_sample"] ge).
 
+Definition header_sample_t: P4Type := ltac:(get_type "header_sample_t" ge).
+Definition metadata_t: P4Type := ltac:(get_type "metadata_t" ge).
+Definition ingress_intrinsic_metadata_t: P4Type :=
+  ltac:(get_type "ingress_intrinsic_metadata_t" ge).
+Definition ingress_intrinsic_metadata_from_parser_t: P4Type :=
+  ltac:(get_type "ingress_intrinsic_metadata_from_parser_t" ge).
+Definition ingress_intrinsic_metadata_for_deparser_t: P4Type :=
+  ltac:(get_type "ingress_intrinsic_metadata_for_deparser_t" ge).
+Definition ingress_intrinsic_metadata_for_tm_t: P4Type :=
+  ltac:(get_type "ingress_intrinsic_metadata_for_tm_t" ge).
+
+Definition set_field_valid (h: Sval) (fld: ident): Sval :=
+  (update fld (EvalBuiltin.setValid (get fld h)) h).
+
+Record ipv4_rec := {
+    ipv4_version: Sval;
+    ipv4_ihl: Sval;
+    ipv4_diffserv: Sval;
+    ipv4_total_len: Sval;
+    ipv4_identification: Sval;
+    ipv4_flags: Sval;
+    ipv4_frag_offset: Sval;
+    ipv4_ttl: Sval;
+    ipv4_protocol: Sval;
+    ipv4_hdr_checksum: Sval;
+    ipv4_src_addr: Sval;
+    ipv4_dst_addr: Sval;
+  }.
+
+Definition hdr (ethernet tcp udp: Sval) (ipv4: ipv4_rec): Sval :=
+  ValBaseStruct
+    [("bridge",
+       ValBaseHeader
+         [("contains_sample", P4Bit_ 8)] (Some true));
+     ("sample",
+       ValBaseHeader
+         [("dmac", P4Bit_ 48);
+          ("smac", P4Bit_ 48);
+          ("etype", P4Bit_ 16);
+          ("srcip", P4Bit_ 32);
+          ("dstip", P4Bit_ 32);
+          ("num_pkts", P4Bit_ 32)] None);
+     ("ethernet", ethernet);
+     ("ipv4",
+       ValBaseHeader
+         [("version", ipv4_version ipv4);
+          ("ihl", ipv4_ihl ipv4);
+          ("diffserv", ipv4_diffserv ipv4);
+          ("total_len", ipv4_total_len ipv4);
+          ("identification", ipv4_identification ipv4);
+          ("flags", ipv4_flags ipv4);
+          ("frag_offset", ipv4_frag_offset ipv4);
+          ("ttl", ipv4_ttl ipv4);
+          ("protocol", ipv4_protocol ipv4);
+          ("hdr_checksum", ipv4_hdr_checksum ipv4);
+          ("src_addr", ipv4_src_addr ipv4);
+          ("dst_addr", ipv4_dst_addr ipv4)] (Some true));
+     ("tcp", tcp);
+     ("udp", udp)].
+
+Definition ig_md (num_pkts: Z) := ValBaseStruct [("num_pkts", P4Bit 32 num_pkts)].
+
 Definition act_sample_spec : func_spec :=
   WITH (* p *),
     PATH p
     MOD (Some [["hdr"]; ["ig_intr_tm_md"]]) [p]
-    WITH hdr,
+    WITH ethernet tcp udp ipv4 ig_intr_tm_md num_pkts,
       PRE
         (ARG []
-        (MEM [(["hdr"], hdr)]
+        (MEM [(["hdr"], hdr ethernet tcp udp ipv4);
+              (["ig_md"], ig_md num_pkts);
+              (["ig_intr_tm_md"], ig_intr_tm_md)]
         (EXT [])))
       POST
         (ARG_RET [] ValBaseNull
-        (MEM [(["hdr"], update "bridge" (bridge_repr 1) hdr)]
+        (MEM [(["hdr"], update "sample"
+                          (sample_repr (ipv4_src_addr ipv4)
+                             (ipv4_dst_addr ipv4) num_pkts)
+                          (update "bridge" (bridge_repr 1)
+                             (hdr ethernet tcp udp ipv4)));
+              (["ig_md"], ig_md num_pkts);
+              (["ig_intr_tm_md"], update "mcast_grp_a" (P4Bit 16 1) ig_intr_tm_md)]
         (EXT []))).
 
 Lemma act_sample_body:
   func_sound ge act_sample_fundef nil act_sample_spec.
 Proof.
   start_function.
-  do 7 step.
-Abort.
+  unfold hdr.
+  simpl.
+  do 10 step.
+  entailer.
+Qed.
